safety.thy
@@ -38,12 +38,34 @@ proof -
 qed
 
 
+lemma snapshot_smaller:
+  assumes wf: "wellFormed_impl E"
+    and eInfo_def: "(events E .[e]) = Some eInfo"
+    and a2: "i < length (event_executionOrder eInfo)"
+    and a4: "(events E .[fst (event_executionOrder eInfo ! i)]) = Some x2"
+  shows "event_snapshot x2 \<le> event_snapshot eInfo"
+  using wf apply (auto simp add: wellFormed_impl_def wellFormed_def wf_causallyConsistent_def)
+  apply (drule_tac x="(e, eInfo)" in bspec)
+   apply (simp add: eInfo_def in_fmap_entries)
+  apply (auto split: option.splits)
+  apply (drule_tac x="fst (event_executionOrder eInfo ! i)" in bspec)
+  using a2 eInfo_def execution_order_in_snapshot local.wf apply blast
+  using a4 by blast
+
+lemma snapshot_smaller_num:
+  assumes "x \<le> y"
+  shows "snapshot_num x e \<le> snapshot_num y e"
+  using assms apply (auto simp add: less_eq_snapshot_def fmap_entries_def)
+  by (metis fmdom'_notD le0 option.case_eq_if)
+
+
 lemma show_all_states:
   assumes wf: "wellFormed_impl E"
     and p: "\<And>state effectors exec_order snapshot. \<lbrakk>
           state = executeEffectors effectors initialState effector_impl;
           effectors = get_effectors E exec_order;
-          valid_event_sequence exec_order snapshot (happensBeforeE E)
+          valid_event_sequence exec_order snapshot (happensBeforeE E);
+          valid_snapshot E snapshot 
         \<rbrakk> \<Longrightarrow> P state"
   shows "forallStates E P"
 proof (auto simp add: forallStates_def forallEvents_def compose_forward_def fmpred_iff)
@@ -52,103 +74,145 @@ proof (auto simp add: forallStates_def forallEvents_def compose_forward_def fmpr
 
   have 1: "event_state_pre eInfo = executeEffectors (get_effectors E (event_executionOrder eInfo)) initialState effector_impl"
     by (smt eInfo_def compose_forward_def fmdom'I fmdom'_notI fmpred_cases local.wf option.sel wellFormed_def wellFormed_impl_def wf_effector_def)
+
+  have valid_snapshot_eInfo: "valid_snapshot E (event_snapshot eInfo)"
+    using eInfo_def in_fmap_entries local.wf wellFormed_def wellFormed_impl_def wf_valid_snapshots_def by fastforce
+
   show "P (event_state_pre eInfo)"
   proof (rule p[OF 1])
     show "get_effectors E (event_executionOrder eInfo) = get_effectors E (event_executionOrder eInfo)"
       by simp
     show "valid_event_sequence (event_executionOrder eInfo) (event_snapshot eInfo) (happensBeforeE E)"
       using eInfo_def local.wf wf_valid_event_sequence by auto
+    show "valid_snapshot E (event_snapshot eInfo)"
+      by (simp add: valid_snapshot_eInfo)
 
   qed
 
-
   show "P (event_state_post eInfo)"
-  proof (rule p)
-    have post_def: "event_state_post eInfo = executeEffectors (event_effectors eInfo) (event_state_pre eInfo) effector_impl"
-      using wf eInfo_def by (auto simp add: wellFormed_impl_def wellFormed_def wf_effector_def compose_forward_def  )
+  proof (cases "event_effectors eInfo")
+    case Nil
+    text {* if there are no effectors, the post-state is equivalent to the pre-state: *}
+    hence "event_state_post eInfo = event_state_pre eInfo"
+      by (smt append_Nil2 compose_forward_def eInfo_def executeEffectors_split fmdom'I fmdom'_notI fmpred_cases local.wf option.sel wellFormed_def wellFormed_impl_def wf_effector_def)
+    thus "P (event_state_post eInfo)"
+      by (simp add: \<open>P (event_state_pre eInfo)\<close>)
+  next
+    case (Cons e' effs)
+    show "P (event_state_post eInfo)"
+    proof (rule p)
+      have post_def: "event_state_post eInfo = executeEffectors (event_effectors eInfo) (event_state_pre eInfo) effector_impl"
+        using wf eInfo_def by (auto simp add: wellFormed_impl_def wellFormed_def wf_effector_def compose_forward_def  )
 
-    have event_effectors_def: "get_effectors E (map (Pair e) [0..<length (event_effectors eInfo)]) = event_effectors eInfo"
-      by (auto simp add: get_effectors_def compose_forward_def eInfo_def nth_equalityI)
+      have event_effectors_def: "get_effectors E (map (Pair e) [0..<length (event_effectors eInfo)]) = event_effectors eInfo"
+        by (auto simp add: get_effectors_def compose_forward_def eInfo_def nth_equalityI)
 
-    have sorted_before: "sorted_partial' (event_executionOrder eInfo) (happensBeforeE E)"
-      using eInfo_def local.wf valid_event_sequence_def wf_valid_event_sequence by blast
-
-
-    show "event_state_post eInfo = executeEffectors (get_effectors E (event_executionOrder eInfo@map (\<lambda>i. (e,i)) [0..<length (event_effectors eInfo)] )) initialState effector_impl"
-      by (simp add: "1" executeEffectors_split get_effectors_split local.event_effectors_def post_def)
-
-    show "get_effectors E (event_executionOrder eInfo @ map (Pair e) [0..<length (event_effectors eInfo)]) = get_effectors E (event_executionOrder eInfo @ map (Pair e) [0..<length (event_effectors eInfo)])"
-      by simp
-
-    have valid_seq: "valid_event_sequence (event_executionOrder eInfo) (event_snapshot eInfo) (happensBeforeE E)"
-      using eInfo_def local.wf wf_valid_event_sequence by blast
-
-
-    have e_notin_snapshot: "e \<notin> snapshot_events (event_snapshot eInfo)"
-      using wf apply (auto simp add: wellFormed_impl_def wellFormed_def wf_acyclic_def fmap_entries_def)
-      by (metis eInfo_def fmlookup_dom'_iff option.distinct(1) option.sel)
-
-    hence e_notin_exec_order: "(e,i) \<notin> set (event_executionOrder eInfo)" for i
-      using valid_event_sequence_def valid_seq by fastforce
-
-    show "valid_event_sequence (event_executionOrder eInfo @ map (Pair e) [0..<length (event_effectors eInfo)]) (snapshot_update (event_snapshot eInfo) e (length (event_effectors eInfo)) ) (happensBeforeE E)"
-      unfolding valid_event_sequence_def proof (intro conjI)
-
-      show " \<forall>(ea, i)\<in>snapshot_entries (snapshot_update (event_snapshot eInfo) e (length (event_effectors eInfo))).
-                \<forall>i'<i. (ea, i') \<in> set (event_executionOrder eInfo @ map (Pair e) [0..<length (event_effectors eInfo)])"
-        using valid_seq by (auto simp add: valid_event_sequence_def snapshot_update_def fmap_entries_def)
-
-      show "\<forall>(e', i)\<in>set (event_executionOrder eInfo @ map (Pair e) [0..<length (event_effectors eInfo)]).
-         i < snapshot_num (snapshot_update (event_snapshot eInfo) e (length (event_effectors eInfo))) e'"
-        using valid_seq e_notin_exec_order by (auto simp add: valid_event_sequence_def snapshot_update_def fmap_entries_def)
-
-      show "sorted_partial' (event_executionOrder eInfo @ map (Pair e) [0..<length (event_effectors eInfo)]) (happensBeforeE E)"
-        apply (auto simp add: sorted_partial'_def nth_append happensBeforeE_def)
-        using  sorted_before apply (simp add: happensBeforeE_def sorted_partial'_def) 
-         apply (auto simp add: happensBeforeP2_def split: if_splits option.splits)
-         apply (metis e_notin_exec_order eq_fst_iff nth_mem)
-        apply (auto simp add: includedIn_def)
-      proof -
-        fix j i x2
-        assume a0: "\<not> j < length (event_executionOrder eInfo)"
-          and a1: "j < length (event_executionOrder eInfo) + length (event_effectors eInfo)"
-          and a2: "i < length (event_executionOrder eInfo)"
-          and a3: "e \<noteq> fst (event_executionOrder eInfo ! i)"
-          and a4: "(events E .[fst (event_executionOrder eInfo ! i)]) = Some x2"
-          and a5: "j - length (event_executionOrder eInfo) < snapshot_num (event_snapshot x2) e"
-        have "event_snapshot x2 \<le> event_snapshot eInfo"
-          using wf apply (auto simp add: wellFormed_impl_def wellFormed_def wf_causallyConsistent_def)
-          apply (drule_tac x="(e, eInfo)" in bspec)
-          apply (simp add: eInfo_def in_fmap_entries)
-          apply (auto split: option.splits)
-          apply (drule_tac x="fst (event_executionOrder eInfo ! i)" in bspec)
-          using wf apply (auto simp add: wellFormed_impl_def wellFormed_def wf_correct_execution_lists_def compose_forward_def)[1]
-           apply (drule_tac x=e and y=eInfo in fmpredD)
-          using eInfo_def apply simp
-           apply (auto simp add:  valid_event_sequence_def)[1]
-           apply (drule_tac x="event_executionOrder eInfo ! i" in bspec) back
-          using a2 apply simp
+      have sorted_before: "sorted_partial' (event_executionOrder eInfo) (happensBeforeE E)"
+        using eInfo_def local.wf valid_event_sequence_def wf_valid_event_sequence by blast
 
 
-          using  apply blast
+      show "event_state_post eInfo = executeEffectors (get_effectors E (event_executionOrder eInfo@map (\<lambda>i. (e,i)) [0..<length (event_effectors eInfo)] )) initialState effector_impl"
+        by (simp add: "1" executeEffectors_split get_effectors_split local.event_effectors_def post_def)
 
-          find_theorems fmpred
+      show "get_effectors E (event_executionOrder eInfo @ map (Pair e) [0..<length (event_effectors eInfo)]) = get_effectors E (event_executionOrder eInfo @ map (Pair e) [0..<length (event_effectors eInfo)])"
+        by simp
 
-          apply (simp add: a4 in_fmap_entries)
-          apply (auto split: option.splits)
+      have valid_seq: "valid_event_sequence (event_executionOrder eInfo) (event_snapshot eInfo) (happensBeforeE E)"
+        using eInfo_def local.wf wf_valid_event_sequence by blast
 
-           apply (simp add: fmap_entries_def)
 
-          sorry (* using causal consistency *)
-        hence "snapshot_num (event_snapshot x2) e = 0"
-          sorry
-        thus "False"
-          using a5 by linarith
+      have e_notin_snapshot: "e \<notin> snapshot_events (event_snapshot eInfo)"
+        using wf apply (auto simp add: wellFormed_impl_def wellFormed_def wf_acyclic_def fmap_entries_def)
+        by (metis eInfo_def fmlookup_dom'_iff option.distinct(1) option.sel)
+
+      hence e_notin_exec_order: "(e,i) \<notin> set (event_executionOrder eInfo)" for i
+        using valid_event_sequence_def valid_seq by fastforce
+
+      show "valid_snapshot E (snapshot_update (event_snapshot eInfo) e (length effs))"
+        unfolding valid_snapshot_def proof (standard, clarsimp)
+        fix a n
+        assume entry: "(a, n) \<in> snapshot_entries (snapshot_update (event_snapshot eInfo) e (length effs))"
+
+        from valid_snapshot_eInfo
+        obtain eInfo' where pre: "(events E .[a]) = Some eInfo' \<and> n < length (event_effectors eInfo')"
+          if  "(a, n) \<in> snapshot_entries (event_snapshot eInfo)"
+          using that apply (auto simp add: valid_snapshot_def)
+          by (smt case_prodD)
+
+
+
+
+        show "\<exists>eInfo. (events E .[a]) = Some eInfo \<and> n < length (event_effectors eInfo)"
+        proof (cases "(a, n) \<in> snapshot_entries (event_snapshot eInfo)")
+          case True
+          hence pre': "(events E .[a]) = Some eInfo' \<and> n < length (event_effectors eInfo')"
+            using pre by simp
+          thus ?thesis by simp
+        next
+          case False
+          hence a: "a = e" and n: "n = length effs"
+            using entry
+            by (auto simp add: snapshot_update_def fmap_entries_def)
+
+          have "(events E .[a]) = Some eInfo"
+            by (simp add: a eInfo_def)
+
+          moreover have "n < length (event_effectors eInfo)"
+            by (simp add: n local.Cons)
+
+          ultimately show ?thesis by force
+        qed
       qed
+
+
+      show "valid_event_sequence (event_executionOrder eInfo @ map (Pair e) [0..<length (event_effectors eInfo)]) (snapshot_update (event_snapshot eInfo) e (length effs) ) (happensBeforeE E)"
+        unfolding valid_event_sequence_def proof (intro conjI)
+
+        have len_simp: "length (event_effectors eInfo) = Suc (length effs)"
+          by (simp add: local.Cons)
+
+
+        show " \<forall>(ea, i)\<in>snapshot_entries (snapshot_update (event_snapshot eInfo) e (length effs)).
+                \<forall>i'<i. (ea, i') \<in> set (event_executionOrder eInfo @ map (Pair e) [0..<length (event_effectors eInfo)])"
+          using valid_seq by (auto simp add: valid_event_sequence_def snapshot_update_def fmap_entries_def len_simp)
+
+
+        show "\<forall>(e', i)\<in>set (event_executionOrder eInfo @ map (Pair e) [0..<length (event_effectors eInfo)]).
+         i < snapshot_num (snapshot_update (event_snapshot eInfo) e (length effs)) e'"
+          using valid_seq e_notin_exec_order by (auto simp add: valid_event_sequence_def snapshot_update_def fmap_entries_def len_simp)
+
+        show "sorted_partial' (event_executionOrder eInfo @ map (Pair e) [0..<length (event_effectors eInfo)]) (happensBeforeE E)"
+          apply (auto simp add: sorted_partial'_def nth_append happensBeforeE_def)
+          using  sorted_before apply (simp add: happensBeforeE_def sorted_partial'_def) 
+           apply (auto simp add: happensBeforeP2_def split: if_splits option.splits)
+           apply (metis e_notin_exec_order eq_fst_iff nth_mem)
+          apply (auto simp add: includedIn_def)
+
+        proof -
+          fix j i x2
+          assume a0: "\<not> j < length (event_executionOrder eInfo)"
+            and a1: "j < length (event_executionOrder eInfo) + length (event_effectors eInfo)"
+            and a2: "i < length (event_executionOrder eInfo)"
+            and a3: "e \<noteq> fst (event_executionOrder eInfo ! i)"
+            and a4: "(events E .[fst (event_executionOrder eInfo ! i)]) = Some x2"
+            and a5: "j - length (event_executionOrder eInfo) < snapshot_num (event_snapshot x2) e"
+
+          have "snapshot_num (event_snapshot eInfo) e = 0"
+            by (simp add: e_notin_snapshot fmdom'_notD)
+
+          have "event_snapshot x2 \<le> event_snapshot eInfo"
+            using a2 a4 eInfo_def local.wf snapshot_smaller by auto
+          hence "snapshot_num (event_snapshot x2) e = 0"
+            using `snapshot_num (event_snapshot eInfo) e = 0`
+            by (metis le_zero_eq snapshot_smaller_num)
+          thus "False"
+            using a5 by linarith
+        qed
+      qed
+
     qed
   qed
 qed
-
 
 (*
 definition wf_effector :: "('operation, 'operation_result, 'operation_effector, 'state)execution \<Rightarrow> 'state \<Rightarrow> ('operation_effector, 'state) effector_function \<Rightarrow> bool" where
@@ -162,12 +226,213 @@ events execution |> fmpred (\<lambda>e eInfo.
 "
 *)
 
-lemma 
+lemma includedIn_snapshot_events: "includedIn e n snapshot \<Longrightarrow> e\<in>snapshot_events snapshot"
+  by (auto simp add: includedIn_def fmdom'I split: option.splits)
+
+
+lemma valid_snapshot_includedIn:
+  assumes "valid_snapshot E snapshot"
+and "includedIn e n snapshot"
+shows "\<exists>eInfo. (events E.[e]) = Some eInfo \<and> n < length (event_effectors eInfo)"
+  using assms  apply (auto simp add: valid_snapshot_def includedIn_def fmap_entries_def)
+  by (metis (no_types, lifting) Suc_leI assms(2) includedIn_snapshot_events less_le_trans not_less0 option.case_eq_if)
+
+lemma showCases: "\<lbrakk>x = None \<Longrightarrow> A; \<And>y. x = Some y \<Longrightarrow> P y\<rbrakk> \<Longrightarrow> (case x of None \<Rightarrow> A | Some y \<Rightarrow> P y)"
+  by (auto split: option.splits)
+
+lemma wellformed_generator:
+  assumes wf: "wellFormed_impl E"
+    and e: "(events E.[e]) = Some eInfo"
+  shows "generator_impl (event_operation eInfo) e (event_state_pre eInfo) = (event_result eInfo, event_effectors eInfo)"
+  using wf  apply (auto simp add: wellFormed_impl_def wellFormed_def wf_generator_def compose_forward_def)
+  using e by auto
+
+lemma set_maps: "set (List.maps f xs) = \<Union>( (set \<circ> f) ` set xs)"
+  apply (induct xs)
+  by (auto simp add: maps_simps)
+
+
+lemma maps_sorted_list_of_set:
+  assumes "finite S"
+  shows "set (List.maps f (sorted_list_of_set S)) = \<Union>(set ` f ` S)"
+  by (simp add: assms set_maps)
+
+lemma sorted_list_of_set2_same: "sorted_list_of_set2 = sorted_list_of_set"
+  by (simp add: sorted_list_of_set2_def sorted_list_of_set_def)
+
+
+lemma maps_sorted_list_of_set2:
+  assumes "finite S"
+  shows "set (List.maps f (sorted_list_of_set2 S)) = \<Union>(set ` f ` S)"
+  by (simp add: assms maps_sorted_list_of_set sorted_list_of_set2_same)
+
+lemma wf_effector_pre:
+  assumes wf: "wellFormed_impl E" 
+    and e: "(events E.[e]) = Some eInfo"
+  shows "event_state_pre eInfo = executeEffectors (get_effectors E (event_executionOrder eInfo)) initialState effector_impl"
+  using wf e  by (auto simp add: wellFormed_impl_def wellFormed_def wf_effector_def compose_forward_def)
+
+
+lemma wf_effector_post:
+  assumes wf: "wellFormed_impl E" 
+    and e: "(events E.[e]) = Some eInfo"
+  shows"event_state_post eInfo = executeEffectors (event_effectors eInfo) (event_state_pre eInfo) effector_impl"
+using wf e  by (auto simp add: wellFormed_impl_def wellFormed_def wf_effector_def compose_forward_def)
+
+lemma filter_finite: "finite S \<Longrightarrow> finite (Set.filter P S)"
+  by (auto simp add: Set.filter_def)
+
+lemma dest_keys_finite_pre[simp]:
+  assumes wf: "wellFormed_impl E"
+    and e: "(events E.[e]) = Some eInfo"
+  shows "finite (dest_keys (ref_state (event_state_pre eInfo) ref))"
+  using wf_effector_pre[OF wf, OF e] apply (auto simp add: ref_state_def split: option.splits)
+proof -
+
+  have h: "\<lbrakk>(state_refs (executeEffectors effs S effector_impl) .[ref]) = Some x; \<And>x. (state_refs S.[ref]) = Some x \<Longrightarrow> finite (dest_keys x)\<rbrakk> \<Longrightarrow> finite (dest_keys x)" for effs x S
+  proof  (induct effs arbitrary: S x)
+    case Nil
+    then show ?case by (auto simp add: executeEffectors_def initialState_def)
+  next
+    case (Cons a effs)
+    from `(state_refs (executeEffectors (a # effs) S effector_impl) .[ref]) = Some x`
+    show ?case 
+      apply (auto simp add: executeEffectors_def initialState_def)
+      apply (fold executeEffectors_def)
+      apply (erule Cons.hyps)
+      using `\<And>x. (state_refs S .[ref]) = Some x \<Longrightarrow> finite (dest_keys x)`
+      apply (auto simp add: effector_impl_def inUse_update_def s_update_inref_def s_update_ref_def ref_state_def Set.filter_def  split: operation_effector.splits if_splits option.splits)
+      done
+  qed
+  show "finite (dest_keys x2)"
+    if c0: "event_state_pre eInfo = executeEffectors (get_effectors E (event_executionOrder eInfo)) initialState effector_impl"
+      and c1: "(state_refs (executeEffectors (get_effectors E (event_executionOrder eInfo)) initialState effector_impl) .[ref]) = Some x2"
+    for  x2
+    using c1 proof (rule h)
+    show "\<And>x. (state_refs initialState .[ref]) = Some x \<Longrightarrow> finite (dest_keys x)"
+      by (simp add: initialState_def)
+  qed
+qed
+
+
+text {* First establish some general facts: 
+How does the state depend on executed effectors (depending on snapshot)
+and which operations can generate which effectors... *}
+
+
+lemma safety_inv1:
   assumes wf: "wellFormed_impl E"
   shows "invariant1 E"
-  unfolding invariant1_def proof (rule show_all_states[OF wf])
+  unfolding invariant1_def compose_forward_def proof (rule show_all_states[OF wf])
+
+  show "\<forall>[r\<mapsto>rState]\<in>state_refs state.
+              \<forall>(k, u)\<in>dest_keys rState.
+                 case k of 
+                   None \<Rightarrow> True 
+                 | Some inref \<Rightarrow> (
+                     case state_inrefs state .[inref] of 
+                         None \<Rightarrow> False 
+                       | Some inrefState \<Rightarrow> (r, u) \<in> two_phase_set_get (rev_refs inrefState))"
+    if c0: "state = executeEffectors effectors initialState effector_impl"
+      and c1: "effectors = get_effectors E exec_order"
+      and c2: "valid_event_sequence exec_order snapshot (happensBeforeE E)"
+      and snapshot_valid: "valid_snapshot E snapshot"
+    for  state effectors exec_order snapshot
+  proof (standard+, auto split: option.splits)
+    fix ref refState u inref
+    assume a0: "(state_refs state .[ref]) = Some refState"
+      and a1: "(Some inref, u) \<in> dest_keys refState"
+
+    text {* Since we have an inref in the destination keys, there must be a corresponding event in the snapshot... *}
+
+    (* from `(Some inref, u) \<in> dest_keys refState` *)
+    have "case events E.[u] of
+            None \<Rightarrow> False
+          | Some uInfo \<Rightarrow>
+           event_operation uInfo = init ref inref \<and> includedIn u 2 snapshot
+         \<or> (\<exists>ref'. event_operation uInfo = assign ref ref' 
+            \<and> (case state_refs (event_state_pre uInfo).[ref'] of 
+                   None \<Rightarrow> False
+                 | Some ref'_state \<Rightarrow> mv_reg_get1' (dest_keys ref'_state) = Some inref  \<and> includedIn u 1 snapshot ))"
+        (* TODO and there does not exists an event after u overriding the assignment. *)
+    proof -
+      have "length exec_order  = length effectors"
+        using c1 by (simp add: get_effectors_def compose_forward_def)
+
+      text {* The only way to change the dest_keys is via a effector_ref_dest_keys_assign effector. *}
+      obtain oldUids 
+        where "effector_ref_dest_keys_assign ref (Some inref) u oldUids \<in> set effectors"
+        sorry
+
+      from this obtain eff_i 
+        where eff_i_def: "effectors ! eff_i = effector_ref_dest_keys_assign ref (Some inref) u oldUids" and "eff_i < length effectors"
+        by (meson in_set_conv_nth)
+
+      text {* the effector must come from the exec order *}
+      from this obtain eff_e eff_n
+        where "exec_order ! eff_i = (eff_e, eff_n)" and "eff_i < length exec_order"
+        using \<open>length exec_order = length effectors\<close> by fastforce
 
 
-qed
+      text {* so the effector must be i the snapshot: *}
+      have "includedIn eff_e eff_n snapshot"
+        using `valid_event_sequence exec_order snapshot (happensBeforeE E)`
+        apply (simp add: valid_event_sequence_def)
+        using \<open>eff_i < length exec_order\<close> \<open>exec_order ! eff_i = (eff_e, eff_n)\<close> includedIn_def nth_mem by fastforce
+
+      text {* The event eff_e must exist. *}
+      obtain eff_e_info where eff_e_info_def: "(events E.[eff_e]) = Some eff_e_info"
+        using `includedIn eff_e eff_n snapshot` snapshot_valid
+        apply (auto simp add: valid_snapshot_def includedIn_def fmap_entries_def split: nat.splits option.splits)
+        by (meson fmdom'I)
+
+      text {* The event eff_e must have generated the effect. *}
+      have eff_e_info_effectors: "event_effectors eff_e_info ! eff_n = effector_ref_dest_keys_assign ref (Some inref) u oldUids"
+        using `effectors = get_effectors E exec_order` eff_i_def by (auto simp add: get_effectors_def compose_forward_def \<open>eff_i < length exec_order\<close> \<open>exec_order ! eff_i = (eff_e, eff_n)\<close> eff_e_info_def)
+
+      have eff_n_range: "eff_n < length (event_effectors eff_e_info)"
+        using `includedIn eff_e eff_n snapshot` `valid_snapshot E snapshot` eff_e_info_def
+        apply (auto simp add: includedIn_def valid_snapshot_def fmap_entries_def split: option.splits)
+        using \<open>includedIn eff_e eff_n snapshot\<close> snapshot_valid valid_snapshot_includedIn by fastforce
+
+      find_theorems "events E .[u]"
+
+      have eff_e_info_effectors_set: "effector_ref_dest_keys_assign ref (Some inref) u oldUids \<in> set (event_effectors eff_e_info)"
+        using eff_e_info_effectors eff_n_range nth_inset by fastforce
+
+
+      have dest_keys_fin[simp]: "finite (dest_keys (ref_state (event_state_pre eff_e_info) x))" for x
+        using eff_e_info_def local.wf by auto
+
+
+      have "u = eff_e"
+        using eff_e_info_effectors_set wellformed_generator[OF wf, OF eff_e_info_def, symmetric]
+        by (auto simp add: generator_impl_def compose_forward_def inref_inuse_enable_def outref_update_def return_def ref_reset_targets_def Let_def 
+                inref_rev_refs_add_def inref_rev_refs_remove_def  ref_dest_keys_assign_def maps_sorted_list_of_set2 skip_def
+                split: operation.splits option.splits)
+
+      text {* Now distinguish the cases how the effect could have been generated via case distinction over the different operations. *}
+      show " case events E .[u] of None \<Rightarrow> False
+            | Some uInfo \<Rightarrow>
+                event_operation uInfo = init ref inref \<and> includedIn u 2 snapshot \<or>
+                (\<exists>ref'. event_operation uInfo = assign ref ref' \<and>
+                        (case state_refs (event_state_pre uInfo) .[ref'] of None \<Rightarrow> False | Some ref'_state \<Rightarrow> mv_reg_get1' (dest_keys ref'_state) = Some inref \<and> includedIn u 1 snapshot)) "
+      proof (simp add: \<open>u = eff_e\<close> eff_e_info_def)
+        show "event_operation eff_e_info = init ref inref \<and> includedIn eff_e 2 snapshot 
+             \<or> (\<exists>ref'. event_operation eff_e_info = assign ref ref' \<and>
+                  (case state_refs (event_state_pre eff_e_info) .[ref'] of 
+                         None \<Rightarrow> False 
+                       | Some ref'_state \<Rightarrow> mv_reg_get1' (dest_keys ref'_state) = Some inref \<and> includedIn u 1 snapshot))"
+
+
+
+    show "False" if "(state_inrefs state .[inref]) = None"
+
+      sorry
+    show "(ref, u) \<in> two_phase_set_get (rev_refs x2a)" if "(state_inrefs state .[inref]) = Some x2a" for x2a
+      sorry
+
+
+  qed
 
 end
